examples/refinement/LowComp.fst
@@ -25,7 +25,6 @@ let lstate_as_state h  = fun (b1, b2) -> (B.get h b1 0, B.get h b2 0)
 
 
 
-// works
 type lcomp 'a (c : comp 'a) = 
     (ls:lstate) ->
     Stack 'a
@@ -39,28 +38,58 @@ type lcomp 'a (c : comp 'a) =
                     snd res == s1 /\ fst res == r )))
 
 
-// works with trial post
-let lcomp_wp1 (a:Type) (wp : state -> (a * state -> Type) -> Type) (c : comp_wp a wp) = 
-     (ls:lstate) ->
-     Stack a
-       (requires (fun h -> well_formed h ls))
-       (ensures  (fun h r h' -> 
-                    well_formed h' ls /\
-                    modifies (loc_union (loc_buffer (fst ls)) (loc_buffer (snd ls))) h h'))
 
 
-// Assertion failed ..
-let lcomp_wp2 (a:Type) (wp : state -> (a * state -> Type) -> Type) (c : comp_wp a wp) = 
+let lcomp_wp (a:Type) (wp : state -> (a * state -> Type) -> Type) (c : comp_wp a wp) = 
      (ls:lstate) ->
      Stack a
        (requires (fun h -> well_formed h ls))
        (ensures  (fun h r h' -> 
                     well_formed h' ls /\
                     modifies (loc_union (loc_buffer (fst ls)) (loc_buffer (snd ls))) h h' /\
+                   
                     (let s0 = lstate_as_state h ls in 
-                     let s1 = lstate_as_state h' ls in
-                     let res = c s0 in True )))
-                     // wp s0 (fun _ -> True) )))
-                     // snd res == s1 /\ fst res == r 
+                     wp s0 (fun _ -> True) /\
+                     (let res = c s0 in
+                     snd res == lstate_as_state h' ls /\ fst res == r)))) 
+
+let lcomp_p (a:Type) pre post (c : comp_p a pre post) = 
+    (ls:lstate) ->
+    Stack a
+      (requires (fun h -> well_formed h ls))
+      (ensures  (fun h r h' -> 
+                   well_formed h' ls /\
+                   modifies (loc_union (loc_buffer (fst ls)) (loc_buffer (snd ls))) h h' /\
+                     
+                   (let s0 = lstate_as_state h ls in 
+                     pre s0 /\
+                     (let res = c s0 in
+                     snd res == lstate_as_state h' ls /\ fst res == r)))) 
 
 
+let reif (#a:Type) (wp:state -> (a * state -> Type) -> Type) (c : unit -> HIGH a wp) : 
+  comp_wp a wp  = reify (c ())
+
+
+let lcomp_r (a:Type) (wp:state -> (a * state -> Type) -> Type) (c : unit -> HIGH a wp) = 
+  (ls:lstate) ->
+    Stack a
+      (requires (fun h -> well_formed h ls))
+      (ensures  (fun h r h' -> 
+                   well_formed h' ls /\
+                   modifies (loc_union (loc_buffer (fst ls)) (loc_buffer (snd ls))) h h' /\
+                   (let s0 = lstate_as_state h ls in 
+                    wp s0 (fun _ -> True) /\
+                    (let res = reif wp c s0 in
+                     // let res = reify (c ()) s0 in XXX using reify directly fails
+                     snd res == lstate_as_state h' ls /\ fst res == r))))
+
+
+(* DSL for low computations *)
+
+let lreturn (#a:Type) (x:a) : lcomp_wp a (return_wp x) (hreturn' x) = fun ls -> x
+
+let lbind (#a:Type) (#b:Type) #wp1 #wp2 (#c1:comp_wp a wp1) (#c2:(x:a -> comp_wp b (wp2 x))) 
+    (m : lcomp_wp a wp1 c1) (f : (x:a) -> lcomp_wp b (wp2 x) (c2 x)) : 
+    lcomp_wp b (bind_wp wp1 wp2) (hbind' c1 c2) = 
+    fun s -> let a = m s in f a s
